---
title: "Moments of the Beta Kernel"
author: "Michael Gordy"
format: html
editor: visual
---

\newcommand{\indicator}[1]{\mathbb{1}_{\{#1\}}}
\newcommand{\betaa}{a}
\newcommand{\betab}{b}
\newcommand{\E}{\mathbb{E}}
\newcommand{\R}{\mathbb{R}}
\newcommand{\Q}{\mathbb{Q}}
\newcommand{\bigO}{\mathcal{O}} 
\newcommand{\N}{\mathbb{N}}

We seek solutions to the moments and cross-moments of the transformed PIT values when the kernel densities take the form
$$
g_\nu(u) = (\alpha_2-\alpha_1)^{1-\betaa-\betab} (u-\alpha_1)^{\betaa-1} (\alpha_2-u)^{\betab-1} \indicator{\alpha_1\leq u\leq\alpha_2}
$$
for parameters $(\betaa>0, \betab>-1/2)$ and $0\leq\alpha_1< \alpha_2\leq1$. We draw upon the websites [FWC](https://functions.wolfram.com) and [DLMF](https://dlmf.nist.gov/), and the books *Atlas of Functions* ("AF") by \citet{bib:atlasfunctions} and *Table of Integrals, Series, and Products* by \citet{bib:gradryz7} ("GR").

Coding is facilitated by computing moments in terms of the moments of standardized beta kernels with $\alpha_1=0,\alpha_2=1$. Let $\tilde{\nu}$ denote a beta$(\betaa,\betab)$ kernel scaled to $[0,1]$ and let $\tilde{W}=G_{\tilde{\nu}}(U)$ for $U\sim\text{Uniform}(0,1)$.  The uncentered moments of $W$ can be obtained as:
\begin{equation}
    \E[W^k] = \begin{cases}
      (\alpha_2-\alpha_1)\E[\tilde{W}^k] + (1-\alpha_2)G_{\tilde{\nu}}(1)^k & \text{if } \alpha_2 < 1 \\
      (1-\alpha_1)\E[\tilde{W}^k] & \text{if } \alpha_2 = 1 .
      \end{cases}
\end{equation}
Proposition \ref{prop:tailbehavior} guarantees that $\lim_{y\rightarrow1} (1-y)G_{\tilde{\nu}}(y)^k=0$ for $k=1,2$, so the expression in the $\alpha_2=1$ case is simply the limit of the expression in the $\alpha_2<1$ case. 

By \citet[8.17.7-8]{bib:DLMF}, the kernel function $G_{\tilde{\nu}}(u)=B(u; \betaa,\betab)$ can be expressed in terms of the Gauss hypergeometric function, ${_2}F_1$, in two equivalent forms: 
\begin{align}
B(u; \betaa,\betab)  &= \frac{u^\betaa}{\betaa}{_2}F_1(\betaa, 1-\betab; \betaa+1; u)  (\#eq:incbetastandard) \\
                &= \frac{u^\betaa(1-u)^\betab}{\betaa} {_2}F_1(1, \betaa+\betab; \betaa+1; u).  (\#eq:incbetavar)
\end{align}
We will use each of these forms below.

The two forms are equivalent at $b=0$. Standard algorithms for the incomplete beta  function are numerically unstable for $\betab\approx 0$ in the neighborhood of $p=1$. For the interesting special case of $\betab=0$ and $\betaa\in\Q^+$, \citet[Theorem 1]{bib:gonzalezSantander} provides a finite series expansion in elementary functions.

The first moment of $\tilde{W}$ is 
$$
  \E[\tilde{W}] = \int_0^1 (1-u)g_{\tilde{\nu}}(u)\,du = B(\betaa,1+\betab) 
$$
Since $\betab>-1/2$, this expression presents no difficulties for our application.

Say we have two beta variables with (possibly) different parameters $(\betaa_i,\betab_i)$ for $i=1,2$. Let $\tilde{G}_i$ denote the transform function for kernel $i$. To get cross-moments and second moments, we need the integral
\begin{align}
   \mbox{}& M(\betaa_1,\betab_1,\betaa_2,\betab_2) = \int_0^1 (1-u) \tilde{g}_1(u) \tilde{G}_2(u) du \label{eq:defineM} \\ 
  &= \frac{B(\betaa_1+\betaa_2,1+\betab_1)}{\betaa_2}
             {_3}F_2(\betaa_2,\betaa_1+\betaa_2,1-\betab_2; 1+\betaa_2, 1+\betaa_1+\betaa_2+\betab_1; 1) \label{eq:MoneA} \\
  &= \frac{B(\betaa_1+\betaa_2,1+\betab_1+\betab_2)}{\betaa_2}
             {_3}F_2(1,\betaa_1+\betaa_2,\betaa_2+\betab_2; 1+\betaa_2, 1+\betaa_1+\betaa_2+\betab_1+\betab_2; 1) \label{eq:MoneB} 
\end{align}
\noindent The two forms come from application of GR 7.512.5 to (\@ref(eq:incbetastandard)) and (\@ref(eq:incbetavar)), respectively.   When calculated from its series expansion, equation \eqref{eq:MoneA} will be numerically stable whenever $\betab_2\leq0$ whereas \eqref{eq:MoneB} will be numerically stable whenever $\betab_2>0$.

There are numerous special cases for which ${_3}F_2(1)$ has known closed-form solution. 

## Case $\betab_1=0$
When $b_1=0$ and $\betab_2\neq0$, we apply FWC 07.27.03.0119.01 to \eqref{eq:incbetastandard} to obtain
\begin{equation}
M(\betaa_1,0,\betaa_2,\betab_2) = \frac{1}{\betaa_1}\left(B(\betaa_2, \betab_2) - B(\betaa_1+\betaa_2, \betab_2)\right)
\end{equation}
When $b_1=\betab_2=0$, we instead apply FWC 07.27.03.0035.01 to \eqref{eq:MoneB}:
\begin{equation}
M(\betaa_1,0,\betaa_2,0) 
     = \frac{1}{\betaa_1}\left(\psi(\betaa_1+\betaa_2)-\psi(\betaa_2)\right)
\end{equation}
where $\psi$ is the digamma function.  One can derive this by noting that FWC 06.14.26.0001.01 and 06.18.06.0004.01 together imply the limit
\[
    \lim_{b\rightarrow0} \left(\frac{1}{b}-B(a,b)\right) = \psi(a)+\gamma
\]
where $\gamma$ is Euler's gamma.

## Case $\betab_1=n\in\N$
\label{sec:bonenatural}
Binomial expansion of the term $(1-u)^{\betab_1}$ in the integral form \eqref{eq:defineM} of $M$ leads to
\begin{equation}
    M(\betaa_1,n,\betaa_2,\betab_2)=
    \sum_{k=0}^n (-1)^k\binom{n}{k} M(\betaa_1+k,0,\betaa_2,\betab_2)
\end{equation}
This approach would be practical for small values of $n$.

## Case $\betaa_2=n\in\N$
For the moment, assume $\betab_2\neq0$. We have from FWC 06.19.03.0003.01:
\begin{equation}
  B(u; n, \betab) = B(n,\betab)\left(
              1-(1-u)^\betab\sum_{k=0}^{n-1}\frac{(\betab)_k u^k}{k!}\right)
\end{equation}
where $(b)_k$ is Pochhammer's notation defined recursively by $(b)_0=1$, $(b)_{m+1}=(b+m)\cdot (b)_m$.
This leads to 
\begin{equation}
\label{eq:betaaaN}
 M(\betaa_1,\betab_1,n,\betab_2) = 
   \frac{(n-1)!}{(\betab_2)_n}\left(B(\betaa_1,1+\betab_1)
   - \sum_{k=0}^{n-1}\frac{(\betab_2)_k}{k!}
     B(\betaa_1+k,1+\betab_1+\betab_2)\right).
\end{equation}
This can be computed more effectively in recursive form:
\begin{align}
    M(\betaa_1,\betab_1,1,\betab_2) &=
    \frac{1}{\betab_2}\left(B(\betaa_1, 1+\betab_1) -
     B(\betaa_1, 1+\betab_1+\betab_2)\right) \label{eq:Mrecursestop}
    \\
    M(\betaa_1,\betab_1,m+1,\betab_2) &= 
    \frac{1}{\betab_2+m}\left(m\; M(\betaa_1,\betab_1,m,\betab_2)-B(\betaa_1+m, 1+\betab_1+\betab_2)\right) \label{eq:Mrecursenext}
\end{align}

To take the limit of \eqref{eq:Mrecursestop} as $\betab_2\rightarrow0$, we have by FWC 06.18.06.0013.01 that 
\[ B(a,b+z) = B(a,b)(1+ z(\psi(b+1)-\psi(a+b+1)) + \bigO(z^2)) \]
which implies 
\begin{equation}
 \label{eq:Monerecursestopzero}
    M(\betaa_1,\betab_1,1,0) = 
     B(\betaa_1,1+\betab_1)\left(\psi(1+\betaa_1+\betab_1) - \psi(1+\betab_1)\right)
\end{equation}
Observe that \eqref{eq:Mrecursenext} is well-behaved at $\betab_2=0$.

\subsection{Case $\betab_2=n\in\N$}
We have from FWC 06.19.03.0001.01:
\begin{equation}
\label{eq:Bxam}
  B(u;\betaa, 1+m) = B(\betaa,1+m)\,u^\betaa \sum_{k=0}^m\frac{(\betaa)_k (1-u)^k}{k!}
\end{equation}
Substituting into the integral for $M$:
\begin{equation}
 M(\betaa_1,\betab_1,\betaa_2,n) = \frac{(n-1)!}{(\betaa_2)_n} 
   \sum_{k=0}^{n-1}\frac{(\betaa_2)_k}{k!} B(\betaa_1+\betaa_2,\betab_1+k+1).
\end{equation}
This could also be expressed compactly in recursive form.  An especially simple subcase is 
\begin{equation}
\label{eq:Mbetatwoisone}
 M(\betaa_1,\betab_1,\betaa_2,1) = \frac{1}{\betaa_2} B(\betaa_1+\betaa_2,\betab_1+1).
\end{equation}


\subsection{Contribution of PIT values above $\alpha_2$ to expected value}
\label{app:uppertailcontribution}
\noteM[inline]{I kind of made a mess of this, but it could easily be turned into a more formal demonstration that we satisfy the condition of Prop \ref{prop:tailbehavior} if $\betab>1/2$. I propose to leave it here for now in case some use arises.}
\noteA[inline]{This seems necessary to retain.}

PIT values above $\alpha_2$ contribute to $\E[W]$ in the term $(1-\alpha_2)G_\nu(\alpha_2)$.  In this appendix we show that
\[
\lim_{y\rightarrow 1} (1-y)G_\nu(y) = 0\;\text{for all } b>-1/2.
\]
Since the incomplete beta function is decreasing in $b$, we need only verify the result for $b=-1/2$.  Using \eqref{eq:incbetavar}, we have
\[
(1-y)B(y; a,-1/2) = \frac{y^\betaa(1-y)^{1/2}}{\betaa}
  {_2}F_1(1, \betaa-1/2; \betaa+1; y) 
\]
By FWC 07.23.03.0002.01,
\[
  {_2}F_1(1, \betaa-1/2; \betaa+1; 1) = 2\betaa.
\]
As the incomplete beta is nonnegative, it follows that
\[
0\leq \lim_{y\rightarrow 1} (1-y)B(y; a, b) \leq \lim_{y\rightarrow 1} 2y^\betaa(1-y)^{1/2} =  0
\]
for all $b>-1/2$.
